FStar.Algebra.Classes.Fractions.fst
@@ -1,0 +1,111 @@
+module FStar.Algebra.Classes.Fractions
+
+open FStar.Algebra.Classes.Equatable
+open FStar.Algebra.Classes.Grouplikes
+open FStar.Algebra.Classes.Ringlikes
+
+module TC = FStar.Tactics.Typeclasses
+
+//instance semiring_of_integral_domain t {| d: integral_domain t |} = d.commutative_ring.ring.semiring
+
+//instance has_one_of_id t {| d: integral_domain t |} = d.commutative_ring.mul_comm_monoid.mul_monoid 
+instance eq_of_id t {| d: integral_domain t |} : equatable t 
+  = d.commutative_ring.ring.semiring.add_comm_monoid.add_monoid.add_semigroup.has_add.eq 
+
+instance has_zero_of_id t {| d: integral_domain t |} = d.commutative_ring.ring.semiring.add_comm_monoid.add_monoid.has_zero
+
+instance has_one_of_id t {| d: integral_domain t |} = d.commutative_ring.mul_comm_monoid.mul_monoid.has_one
+
+type nonzero_of #t (d: integral_domain t) = x:t{x<>zero}
+
+type fraction #t (d: integral_domain t) = 
+  | Fraction : (num:t) -> (den: nonzero_of d) -> fraction #t d
+
+let ( / ) (#t:Type) {| d: integral_domain t |} (x:t) (y:nonzero_of d) : fraction d =
+  Fraction x y
+ 
+let fraction_one t {| d: integral_domain t |} =    
+  let one:t = one in
+  symmetry zero one;
+  one/one
+
+let dec (x: pos) : p:nat{p<<x} = (x - 1) <: int
+
+instance eq_of_nat : equatable nat = {
+  eq = int_equatable.eq;
+  reflexivity = (fun _ -> ());
+  symmetry = (fun _ _ -> ());
+  transitivity = (fun _ _ _ -> ());
+}
+
+private let rec coerce_pos #t (r: semiring t) (x:nat) : t =
+  let one:t = one in
+  let zero:t = zero in
+  let o,l : t&t = zero, one in
+  if x `int_equatable.eq` 0 then o
+  else l + coerce_pos r (dec x)
+
+let ( |- ) #t (r: semiring t) (n: nat) : t = 
+  coerce_pos r n
+
+let product_of_denominators_is_valid_denominator #t {| d: integral_domain t |} (x y: fraction d)
+  : Lemma (x.den * y.den <> (zero <: t)) = Classical.move_requires_2 (d.domain.domain_law) x.den y.den
+
+let semiring_coerce_one #t (r: semiring t) : Lemma ( (r |- 1) = one ) = 
+  let one : t = one in
+  assert ((r|-1) == one + zero);
+  right_add_identity one 
+
+let fraction_eq #t {| d: integral_domain t |} (x y: fraction d) : bool =
+  (x.num * y.den) = (x.den * y.num)
+
+private let fraction_eq_symmetry_aux #t (d: integral_domain t) (x y: fraction d)
+  : Lemma (fraction_eq x y ==> fraction_eq y x) = 
+  mul_commutativity y.num x.den;
+  mul_commutativity x.num y.den;
+  symmetry (x.den*y.num) (x.num*y.den);
+  if fraction_eq x y then
+  trans_lemma [ y.num*x.den;
+                x.den*y.num;
+                x.num*y.den;
+                y.den*x.num ]
+
+let fraction_eq_is_symmetric #t (d:integral_domain t) (x y: fraction d)
+  : Lemma (fraction_eq x y <==> fraction_eq y x) = 
+  fraction_eq_symmetry_aux d x y;
+  fraction_eq_symmetry_aux d y x 
+
+let fraction_eq_is_reflexive #t (d:integral_domain t) (x: fraction d)
+  : Lemma (fraction_eq x x) = mul_commutativity x.num x.den
+ 
+let fraction_eq_is_transitive #t (dom:integral_domain t) (x y z: fraction dom)
+  : Lemma (requires fraction_eq x y /\ fraction_eq y z) (ensures fraction_eq x z) = 
+  let (=) = (eq_of_id t).eq in
+  Classical.forall_intro (eq_of_id t).reflexivity;
+  Classical.forall_intro_3 (Classical.move_requires_3 (eq_of_id t).transitivity);
+  Classical.forall_intro_2 (eq_of_id t).symmetry; 
+  let mul_congruence_3 (x y z:t) 
+    : Lemma (requires x=y) (ensures (x*z = y*z) /\ (z*x = z*y)) 
+    = mul_congruence x z y z; mul_congruence z x z y in
+  let (a,b,c,d,e,f) : (t & t & t & t & t & t) = (x.num, x.den, y.num, y.den, z.num, z.den) in
+  mul_congruence_3 (c*f) (d*e) (a*d);
+  mul_congruence_3 (a*d) (b*c) (d*e);
+  assert ((b*c)*(d*e) = (a*d)*(d*e)); 
+  calc (=) {
+    (b*c)*(d*e); = { mul_associativity (b*c) d e }
+    ((b*c)*d)*e; = { mul_associativity b c d;
+                     mul_congruence_3 ((b*c)*d) (b*(c*d)) e }
+    (b*(c*d))*e; = { mul_commutativity c d; 
+                     mul_congruence_3 (c*d) (d*c) b;
+                     mul_congruence_3 (b*(c*d)) (b*(d*c)) e }
+    (b*(d*c))*e;
+  };
+  calc (=) {
+    (a*d)*(c*f); = { mul_associativity a d (c*f);
+                     mul_associativity d c f;
+                     mul_congruence_3 (d*(c*f)) ((d*c)*f) a }
+    a*((d*c)*f);
+  };
+  
+  admit();
+  () 
